# Saved by TopBraid on Sun Jun 27 12:33:57 CEST 2010
# baseURI: http://purl.org/ontology/infoservice/
# imports: http://purl.org/dc/elements/1.1/
# imports: http://www.w3.org/2003/06/sw-vocab-status/ns
# imports: http://xmlns.com/foaf/0.1/
# imports: http://purl.org/dc/terms/

@prefix category:  <http://dbpedia.org/resource/Category:> .
@prefix dc:      <http://purl.org/dc/elements/1.1/> .
@prefix dcterms:  <http://purl.org/dc/terms/> .
@prefix foaf:    <http://xmlns.com/foaf/0.1/> .
@prefix is:      <http://purl.org/ontology/infoservice/> .
@prefix owl:     <http://www.w3.org/2002/07/owl#> .
@prefix rdf:     <http://www.w3.org/1999/02/22-rdf-syntax-ns#> .
@prefix rdfs:    <http://www.w3.org/2000/01/rdf-schema#> .
@prefix vs:      <http://www.w3.org/2003/06/sw-vocab-status/ns#> .
@prefix xsd:     <http://www.w3.org/2001/XMLSchema#> .

is:   rdf:type owl:Ontology ;
      dc:date "$Date: 2010/06/26 15:57:19 $"^^xsd:string ;
      dc:description """The Information Service Ontology Specification provides basic concepts and properties 
for describing different information services, e.g. Wikipedia, MusicBrainz, Freebase or Discogs, on/ for 
the Semantic Web. This document contains a RDF description of the Information Service Ontology."""@en ;
      dc:title "The Information Service Ontology" ;
      owl:imports foaf: , <http://www.w3.org/2003/06/sw-vocab-status/ns> , dcterms: , dc: ;
      owl:versionInfo "Revision: 0.4.1"@en ;
      foaf:maker <http://foaf.me/zazi#me> .

is:InfoService
      rdf:type owl:Class ;
      rdfs:comment """Short definition: 

	\"An Information Service is a service, which provides (serves) data/knowledge/information somehow.\"

However, this definition is not strong enough to describe the range and domain of an Information Service. Therefore, it is necessary to 
define the term Information Service in a specific context.

Extended definition:

	\"An Information Service is this part of an Information System that serves data/knowledge/information to customers and collects it 
	from its contributors, to manage and store it by optionally using administrators.\"

Please refer also this article[1] about the definition of the term 'Information Service'.

This concept is for linking a piece of information of a specific concept instance (or at least website links or other data representations 
of this concept instance), e.g. a foaf:Agent, a mo:Track or a mo:MusicArtist to a related website of a specific information service (modelled 
as individual of is:InfoService), e.g. Wikipedia, MySpace, MusicBrainz, Discogs, Last.fm, Pandora, BBC, ... . With this concept it is possible 
to describe the underlying information services of that knowledge representation more in detail, so that the client, which consumes that 
'linked data' could choose, which source it likes to use by evaluating the description of the information service of that website link or 
other data representation.


[1] https://infoserviceonto.wordpress.com/2010/06/23/what-is-an-information-service/"""@en ;
      rdfs:isDefinedBy is: ;
      rdfs:label "Information Service"@en ;
      rdfs:subClassOf owl:Thing ;
      vs:term_status "unstable"@en .

is:InfoServiceContributorType
      rdf:type owl:Class ;
      rdfs:comment """This concept is for describing the different contributor types of information services, e.g. expert, 
community or mixed. Please feel free to define further information service contributor types."""@en ;
      rdfs:isDefinedBy is: ;
      rdfs:label "Information Service Contributor Type"@en ;
      rdfs:subClassOf owl:Thing ;
      vs:term_status "testing"@en .

is:InfoServiceQuality
      rdf:type owl:Class ;
      rdfs:comment """This concept is for describing specific quality levels or ratings, e.g. good or bad or more detailed ones, of 
information services. Please feel free to use this concept as hook for more complex and detailed information service quality description 
modellings in sub ontologies. Futhermore, such information service ratings could be done by different information service rating agencies, 
so that the customer of such ratings could select its information service ratings agency of choice."""@en ;
      rdfs:isDefinedBy is: ;
      rdfs:label "Information Service Quality"@en ;
      rdfs:subClassOf owl:Thing ;
      vs:term_status "testing"@en .

is:InfoServiceType
      rdf:type owl:Class ;
      rdfs:comment """This concept is for describing the type of an information service, e.g. 'social network service', 
'recommender service' or 'encyclopedia'. Please feel free to define further information service types for categorisation."""@en ;
      rdfs:isDefinedBy is: ;
      rdfs:label "Information Service Type"@en ;
      rdfs:subClassOf owl:Thing ;
      vs:term_status "unstable"@en .

is:bad
      rdf:type is:InfoServiceQuality ;
      rdfs:isDefinedBy is: ;
      dc:description "This is currently the third worst quality level from the information service quality scale."@en ;
      dc:title "bad"@en .

is:bbc
      rdf:type is:InfoService ;
      rdfs:isDefinedBy is: ;
      dc:description "The largest broadcasting organization in the world. Modelled here as information service."@en ;
      dc:title "BBC"^^xsd:string ;
      foaf:homepage <http://www.bbc.co.uk/> .

is:community
      rdf:type is:InfoServiceContributorType ;
      rdfs:isDefinedBy is: ;
      dc:description "This is the information service type for community driven information services."@en ;
      dc:title "community"@en .

is:discogs
      rdf:type is:InfoService ;
      rdfs:isDefinedBy is: ;
      dc:description """A website and database of information about music recordings, and one of the largest online databases
of electronic music releases and is believed to be the largest online database of releases on vinyl media. Modelled here as
information service."""@en ;
      dc:title "Discogs"^^xsd:string ;
      foaf:homepage <http://www.discogs.com/> .

is:echonest
      rdf:type is:InfoService ;
      rdfs:isDefinedBy is: ;
      dc:description """The Echo Nest provides a series of web based solutions for better search, recommendation and 
interactivity on the music web (including musicial fingerprinting). Modelled here as information service."""@en ;
      dc:title "EchoNest"^^xsd:string .

is:encyclopedia
      rdf:type is:InfoServiceType ;
      rdfs:isDefinedBy is: ;
      dc:description """An encyclopedia is a type of reference work, a compendium holding information from either all branches of 
knowledge or a particular branch of knowledge."""@en ;
      dc:title "encyclopedia"@en .

is:expert
      rdf:type is:InfoServiceContributorType ;
      rdfs:isDefinedBy is: ;
      dc:description "This is the information service type for expert driven information services."@en ;
      dc:title "expert"@en .

is:freebase
      rdf:type is:InfoService ;
      rdfs:isDefinedBy is: ;
      dc:description """An online collection of structured data harvested from many sources. Modelled here as information
service."""@en ;
      dc:title "Freebase"^^xsd:string ;
      foaf:homepage <http://www.freebase.com/> .

is:good
      rdf:type is:InfoServiceQuality ;
      rdfs:isDefinedBy is: ;
      dc:description "This is currently the second best quality level from the information service quality scale."@en ;
      dc:title "good"@en .

is:info_service
      rdf:type owl:ObjectProperty ;
      rdfs:comment """This property could be used to associate a specific owl:Thing typed semantic graph description or especially
a website link, e.g. typed as foaf:Document, to the specific is:InfoService individual. This enables the consumer of this resource
to retrieve more information (descriptions, ratings) about the underlying information service of this resource."""@en ;
      rdfs:domain owl:Thing ;
      rdfs:isDefinedBy is: ;
      rdfs:label "has info service"@en ;
      rdfs:range is:InfoService ;
      owl:InverseOf
              [ rdf:type owl:ObjectProperty ;
                rdfs:label "is info service of"@en
              ] ;
      vs:term_status "unstable"@en .

is:info_service_contributor_type
      rdf:type owl:ObjectProperty ;
      rdfs:comment """With this property it is possible to associate a specific information service contributor type, e.g. expert, 
community or mixed, to an is:InfoService instance."""@en ;
      rdfs:domain is:InfoService ;
      rdfs:isDefinedBy is: ;
      rdfs:label "has info service contributor type"@en ;
      rdfs:range is:InfoServiceContributorType ;
      owl:InverseOf
              [ rdf:type owl:ObjectProperty ;
                rdfs:label "is info service contributor type of"@en
              ] ;
      vs:term_status "testing"@en .

is:info_service_quality
      rdf:type owl:ObjectProperty ;
      rdfs:comment """With this property it is possible to associate a specific quality level or information service rating
to an is:InfoService instance"""@en ;
      rdfs:domain is:InfoService ;
      rdfs:isDefinedBy is: ;
      rdfs:label "has info service quality"@en ;
      rdfs:range is:InfoServiceQuality ;
      owl:InverseOf
              [ rdf:type owl:ObjectProperty ;
                rdfs:label "is info service quality of"@en
              ] ;
      vs:term_status "testing"@en .

is:info_service_type
      rdf:type owl:ObjectProperty ;
      rdfs:comment """With this property it is possible to associate a specific information service type, e.g. 'social network service', 
'recommender service' or 'encyclopedia', to an is:InfoService instance. This property could be used multiple times that means an 
is:InfoService instance could be for example of the information service type 'social network site' and 'recommender system'."""@en ;
      rdfs:domain is:InfoService ;
      rdfs:isDefinedBy is: ;
      rdfs:label "has info service type"@en ;
      rdfs:range is:InfoServiceType ;
      owl:InverseOf
              [ rdf:type owl:ObjectProperty ;
                rdfs:label "is info service type of"@en
              ] ;
      vs:term_status "testing"@en .

is:knowledge_base
      rdf:type is:InfoServiceType ;
      rdfs:isDefinedBy is: ;
      dc:description """A knowledge base is a special kind of database for knowledge management, providing the means for the 
computerized collection, organization, and retrieval of knowledge."""@en ;
      dc:title "knowledge base"@en .

is:lastfm
      rdf:type is:InfoService ;
      rdfs:isDefinedBy is: ;
      dc:description "A popular Internet radio site for streaming music. Modelled here as information service."@en ;
      dc:title "Last.fm"^^xsd:string ;
      foaf:homepage <http://last.fm/> .

is:main_subject
      rdf:type rdf:Property ;
      rdfs:comment """This property is for defining the main subject of an is:InfoService instance that means this 
info service address mainly this concern."""@en ;
      rdfs:domain is:InfoService ;
      rdfs:isDefinedBy "http://purl.org/ontology/infoservice/"@en ;
      rdfs:label "main subject"@en ;
      rdfs:subPropertyOf dcterms:subject ;
      owl:InverseOf
              [ rdf:type rdf:Property ;
                rdfs:label "is main subject of"@en
              ] ;
      vs:term_status "testing"@en .

is:middle
      rdf:type is:InfoServiceQuality ;
      rdfs:isDefinedBy is: ;
      dc:description "This is currently the third best quality level from the information service quality scale."@en ;
      dc:title "middle"@en .

is:mixed
      rdf:type is:InfoServiceContributorType ;
      rdfs:isDefinedBy is: ;
      dc:description """This is the information service type, where both parties - experts and a user community - share 
their knowledge to that information service."""@en ;
      dc:title "mixed"@en .

is:musicbrainz
      rdf:type is:InfoService ;
      rdfs:isDefinedBy is: ;
      dc:description "An open content music database. Modelled here as information service."@en ;
      dc:title "MusicBrainz"^^xsd:string ;
      dcterms:subject <category:Online_music_and_lyrics_databases> , <category:Metadata_registry> , <category:MusicBrainz> , <category:Online_encyclopedias> , <category:Acoustic_fingerprinting> , <category:Library_2.0> , <category:Free_websites> ;
      is:info_service_contributor_type
              is:mixed ;
      is:info_service_quality
              is:good ;
      is:info_service_type
              is:knowledge_base , is:encyclopedia ;
      is:main_subject <category:Music> ;
      foaf:homepage <http://musicbrainz.org/> .

is:myspace
      rdf:type is:InfoService ;
      rdfs:isDefinedBy is: ;
      dc:description """A social networking website with a great pool of musician profiles. Modelled here as information
service."""@en ;
      dc:title "MySpace"^^xsd:string ;
      foaf:homepage <http://www.myspace.com/> .

is:pandora
      rdf:type is:InfoService ;
      rdfs:isDefinedBy is: ;
      dc:description "An automated music recommendation service. Modelled here as information service."@en ;
      dc:title "Pandora"^^xsd:string ;
      foaf:homepage <http://www.pandora.com/> .

is:recommender_service
      rdf:type is:InfoServiceType ;
      rdfs:isDefinedBy is: ;
      dc:description """A recommender service forms or works from a specific type of information filtering system technique 
that attempts to recommend information items (films, television, video on demand, music, books, news, images, web pages, etc) 
that are likely to be of interest to the user."""@en ;
      dc:title "recommender service"@en .

is:social_network_service
      rdf:type is:InfoServiceType ;
      rdfs:isDefinedBy is: ;
      dc:description """A social network service focuses on building and reflecting of social networks or social relations 
among people, e.g., who share interests and/or activities. A social network service essentially consists of a representation 
of each user (often a profile), his/her social links, and a variety of additional services."""@en ;
      dc:title "social network service"@en .

is:spotify
      rdf:type is:InfoService ;
      rdfs:isDefinedBy is: ;
      dc:description "A proprietary peer-to-peer music streaming service. Modelled here as information service."@en ;
      dc:title "Spotify"^^xsd:string ;
      foaf:homepage <http://www.spotify.com/> .

is:useless
      rdf:type is:InfoServiceQuality ;
      rdfs:isDefinedBy is: ;
      dc:description "This is currently the worst quality level from the information service quality scale."@en ;
      dc:title "useless"@en .

is:very_bad
      rdf:type is:InfoServiceQuality ;
      rdfs:isDefinedBy is: ;
      dc:description "This is currently the second worst quality level from the info service quality scale."@en ;
      dc:title "very bad"@en .

is:very_good
      rdf:type is:InfoServiceQuality ;
      rdfs:isDefinedBy is: ;
      dc:description "This is currently the best quality level from the information service quality scale."@en ;
      dc:title "very good"@en .

is:wikipedia
      rdf:type is:InfoService ;
      rdfs:isDefinedBy is: ;
      dc:description "A free, web-based, collaborative, multilingual encyclopedia project. Modelled here as information service."@en ;
      dc:title "Wikipedia"^^xsd:string ;
      foaf:homepage <http://www.wikipedia.org/> .
