# Saved by TopBraid on Sun Jun 20 19:47:09 CEST 2010
# baseURI: http://purl.org/ontology/infoservice/
# imports: http://www.w3.org/2003/06/sw-vocab-status/ns
# imports: http://purl.org/dc/terms/

@prefix category:  <http://dbpedia.org/resource/Category:> .
@prefix dc:      <http://purl.org/dc/elements/1.1/> .
@prefix dcterms:  <http://purl.org/dc/terms/> .
@prefix foaf:    <http://xmlns.com/foaf/0.1/> .
@prefix is:      <http://purl.org/ontology/infoservice/> .
@prefix owl:     <http://www.w3.org/2002/07/owl#> .
@prefix rdf:     <http://www.w3.org/1999/02/22-rdf-syntax-ns#> .
@prefix rdfs:    <http://www.w3.org/2000/01/rdf-schema#> .
@prefix vs:      <http://www.w3.org/2003/06/sw-vocab-status/ns#> .
@prefix xsd:     <http://www.w3.org/2001/XMLSchema#> .

is:   rdf:type owl:Ontology ;
      dc:date "$Date: 2010/06/20 19:37:19 $"^^xsd:string ;
      dc:description """The Information Service Ontology Specification provides basic concepts and properties 
for describing different information services, e.g. Wikipedia, MusicBrainz, Freebase or Discogs, on/ for 
the Semantic Web. This document contains a RDF description of the Information Service Ontology."""^^xsd:string ;
      dc:title "The Information Service Ontology" ;
      owl:imports <http://www.w3.org/2003/06/sw-vocab-status/ns> , dcterms: ;
      owl:versionInfo "Revision: 0.4"^^xsd:string ;
      foaf:maker <http://foaf.me/zazi#me> .

is:InfoService
      rdf:type owl:Class ;
      rdfs:comment "A information service is a service, which provides data somehow. This concept is for linking a information of a specific concept instance (or at least website links or other data representations of this concept instance), e.g. a foaf:Agent, a mo:Track or a mo:MusicArtist to a related website of a specific information service (modelled as individual of is:InfoService), e.g. Wikipedia, MySpace, MusicBrainz, Discogs, Last.fm, Pandora, BBC, ... . With this concept it is possible to describe the underlying info services of that knowledge representation more in detail, so that the client, which consumes that 'linked data' could choose, which source it likes to use by evaluating the description of the info service of that website link or other data representation."^^xsd:string ;
      rdfs:isDefinedBy "http://purl.org/ontology/infoservice/"^^xsd:string ;
      rdfs:label "information service"^^xsd:string ;
      rdfs:subClassOf owl:Thing ;
      vs:term_status "unstable"^^xsd:string .

is:InfoServiceContributorType
      rdf:type owl:Class ;
      rdfs:comment "This concept is for describing the different contributor types of info services, e.g. expert, community or mixed."^^xsd:string ;
      rdfs:isDefinedBy "ttp://purl.org/ontology/infoservice/"^^xsd:string ;
      rdfs:label "info service contributor type"^^xsd:string ;
      rdfs:subClassOf owl:Thing ;
      vs:term_status "testing"^^xsd:string .

is:InfoServiceQuality
      rdf:type owl:Class ;
      rdfs:comment "This concept is for describing specific quality levels, e.g. good or bad or more detailed ones, of info services. Please feel free to use this concept as hook for more complex and detailed information quality description modellings in sub ontologies. Futhermore, such info services ratings could be done by different info service rating agencies, so that the customer of such ratings could select its info service ratings agency of choice."^^xsd:string ;
      rdfs:isDefinedBy "http://purl.org/ontology/infoservice/"^^xsd:string ;
      rdfs:label "info service quality"^^xsd:string ;
      rdfs:subClassOf owl:Thing ;
      vs:term_status "testing"^^xsd:string .

is:InfoServiceType
      rdf:type owl:Class ;
      rdfs:comment "This concept is for describing the type of an info service, e.g. 'social network service', 'recommender service' or 'encyclopedia'."^^xsd:string ;
      rdfs:isDefinedBy "http://purl.org/ontology/infoservice/"^^xsd:string ;
      rdfs:label "info service"^^xsd:string ;
      rdfs:subClassOf owl:Thing ;
      vs:term_status "unstable"^^xsd:string .

is:bad
      rdf:type is:InfoServiceQuality ;
      rdfs:isDefinedBy "http://purl.org/ontology/infoservice/"^^xsd:string ;
      dc:description "This is currently third worst quality level from the info service quality scale."^^xsd:string ;
      dc:title "bad"^^xsd:string .

is:bbc
      rdf:type is:InfoService ;
      rdfs:isDefinedBy "http://purl.org/ontology/infoservice/"^^xsd:string ;
      dc:description "The largest broadcasting organization in the world."^^xsd:string ;
      dc:title "BBC"^^xsd:string ;
      foaf:homepage <http://www.bbc.co.uk/> .

is:community
      rdf:type is:InfoServiceContributorType ;
      rdfs:isDefinedBy "http://purl.org/ontology/infoservice/"^^xsd:string ;
      dc:description "This is the info service type for community driven info services."^^xsd:string ;
      dc:title "community"^^xsd:string .

is:discogs
      rdf:type is:InfoService ;
      rdfs:isDefinedBy "http://purl.org/ontology/infoservice/"^^xsd:string ;
      dc:description "A website  and database  of information about music recordings, and one of the largest online databases of electronic music releases and is believed to be the largest online database of releases on vinyl media."^^xsd:string ;
      dc:title "Discogs"^^xsd:string ;
      foaf:homepage <http://www.discogs.com/> .

is:echonest
      rdf:type is:InfoService ;
      rdfs:isDefinedBy "http://purl.org/ontology/infoservice/"^^xsd:string ;
      dc:description "The Echo Nest provides a series of web based solutions for better search, recommendation and interactivity on the music web (including musicial fingerprinting)."^^xsd:string ;
      dc:title "EchoNest"^^xsd:string .

is:encyclopedia
      rdf:type is:InfoServiceType ;
      rdfs:isDefinedBy "http://purl.org/ontology/infoservice/"^^xsd:string ;
      dc:description "An encyclopedia is a type of reference work, a compendium holding information from either all branches of knowledge or a particular branch of knowledge."^^xsd:string ;
      dc:title "encyclopedia"^^xsd:string .

is:expert
      rdf:type is:InfoServiceContributorType ;
      rdfs:isDefinedBy "http://purl.org/ontology/infoservice/"^^xsd:string ;
      dc:description "This is the info service type for expert driven info services."^^xsd:string ;
      dc:title "expert"^^xsd:string .

is:freebase
      rdf:type is:InfoService ;
      rdfs:isDefinedBy "http://purl.org/ontology/infoservice/"^^xsd:string ;
      dc:description "An online collection of structured data harvested from many sources."^^xsd:string ;
      dc:title "Freebase"^^xsd:string ;
      foaf:homepage <http://www.freebase.com/> .

is:good
      rdf:type is:InfoServiceQuality ;
      rdfs:isDefinedBy "http://purl.org/ontology/infoservice/"^^xsd:string ;
      dc:description "This is currently the second best quality level from the info service quality scale."^^xsd:string ;
      dc:title "good"^^xsd:string .

is:info_service
      rdf:type owl:ObjectProperty ;
      rdfs:comment "This property could be used to associate a specific foaf:Document typed website link to the specific is:InfoService individual. Furthermore, it could also applied on other represenations of data from an info service, e.g. semantic graphs."^^xsd:string ;
      rdfs:domain owl:Thing ;
      rdfs:isDefinedBy "http://purl.org/ontology/infoservice/"^^xsd:string ;
      rdfs:label "has info service"^^xsd:string ;
      rdfs:range is:InfoService ;
      owl:InverseOf
              [ rdfs:label "is info service of"^^xsd:string
              ] ;
      vs:term_status "unstable"^^xsd:string .

is:info_service_contributor_type
      rdf:type owl:ObjectProperty ;
      rdfs:comment "With this property it is possible to associate a specific info service contributor type, e.g. expert, community or mixed, to an is:InfoService instance."^^xsd:string ;
      rdfs:domain is:InfoService ;
      rdfs:isDefinedBy "http://purl.org/ontology/infoservice/"^^xsd:string ;
      rdfs:label "has info service contributor type"^^xsd:string ;
      rdfs:range is:InfoServiceContributorType ;
      owl:InverseOf
              [ rdfs:label "is info service contributor type of"^^xsd:string
              ] ;
      vs:term_status "testing"^^xsd:string .

is:info_service_quality
      rdf:type owl:ObjectProperty ;
      rdfs:comment "With this property it is possible to associate a specific quality level to an is:InfoService instance"^^xsd:string ;
      rdfs:domain is:InfoService ;
      rdfs:isDefinedBy "http://purl.org/ontology/infoservice/"^^xsd:string ;
      rdfs:label "has info service quality"^^xsd:string ;
      rdfs:range is:InfoServiceQuality ;
      owl:InverseOf
              [ rdfs:label "is info service quality of"^^xsd:string
              ] ;
      vs:term_status "testing"^^xsd:string .

is:info_service_type
      rdf:type owl:ObjectProperty ;
      rdfs:comment "With this property it is possible to associate a specific info service type, e.g. 'social network service', 'recommender service' or 'encyclopedia', to an is:InfoService instance. This property could be used multiple times that means an is:InfoService instance could be of the info service type 'social network site' and 'recommender system'."^^xsd:string ;
      rdfs:domain is:InfoService ;
      rdfs:isDefinedBy "http://purl.org/ontology/infoservice/"^^xsd:string ;
      rdfs:label "has info service type"^^xsd:string ;
      rdfs:range is:InfoServiceType ;
      owl:InverseOf
              [ rdfs:label "is info service type of"^^xsd:string
              ] ;
      vs:term_status "testing"^^xsd:string .

is:knowledge_base
      rdf:type is:InfoServiceType ;
      rdfs:isDefinedBy ""^^xsd:string ;
      dc:description "A knowledge base is a special kind of database for knowledge management, providing the means for the computerized collection, organization, and retrieval  of knowledge."^^xsd:string ;
      dc:title "knowledge base"^^xsd:string .

is:lastfm
      rdf:type is:InfoService ;
      rdfs:isDefinedBy "http://purl.org/ontology/infoservice/"^^xsd:string ;
      dc:description "A popular Internet radio site for streaming music."^^xsd:string ;
      dc:title "Last.fm"^^xsd:string ;
      foaf:homepage <http://last.fm/> .

is:main_subject
      rdf:type rdf:Property ;
      rdfs:comment "This property is for defining the main subject of an is:InfoService instance that means this info service address mainly this concern."^^xsd:string ;
      rdfs:domain is:InfoService ;
      rdfs:isDefinedBy "http://purl.org/ontology/infoservice/"^^xsd:string ;
      rdfs:label "main subject"^^xsd:string ;
      rdfs:subPropertyOf dcterms:subject ;
      owl:InverseOf
              [ rdfs:label "is main subject of"^^xsd:string
              ] ;
      vs:term_status "testing"^^xsd:string .

is:middle
      rdf:type is:InfoServiceQuality ;
      rdfs:isDefinedBy "http://purl.org/ontology/infoservice/"^^xsd:string ;
      dc:description "This is currently the third best quality level from the info service quality scale."^^xsd:string ;
      dc:title "middle"^^xsd:string .

is:mixed
      rdf:type is:InfoServiceContributorType ;
      rdfs:isDefinedBy "http://purl.org/ontology/infoservice/"^^xsd:string ;
      dc:description "This is the info service type, where both parties - experts and a user community - share their knowledge to that info service."^^xsd:string ;
      dc:title "mixed"^^xsd:string .

is:musicbrainz
      rdf:type is:InfoService ;
      rdfs:isDefinedBy "http://purl.org/ontology/infoservice/"^^xsd:string ;
      dc:description "An open content music database."^^xsd:string ;
      dc:title "MusicBrainz"^^xsd:string ;
      dcterms:subject "<category:Acoustic_fingerprinting>"^^xsd:string , "<category:MusicBrainz>"^^xsd:string , "<category:Library_2.0>"^^xsd:string , "<category:Online_encyclopedias>"^^xsd:string , "<category:Online_music_and_lyrics_databases>"^^xsd:string , "<category:Free_websites>"^^xsd:string , "<category:Metadata_registry>"^^xsd:string ;
      is:info_service_contributor_type
              is:mixed ;
      is:info_service_quality
              is:good ;
      is:info_service_type
              is:knowledge_base , is:encyclopedia ;
      is:main_subject "<category:Music>"^^xsd:string ;
      foaf:homepage <http://musicbrainz.org/> .

is:myspace
      rdf:type is:InfoService ;
      rdfs:isDefinedBy "http://purl.org/ontology/infoservice/"^^xsd:string ;
      dc:description "A social networking website with a great pool of musician profiles."^^xsd:string ;
      dc:title "MySpace"^^xsd:string ;
      foaf:homepage <http://www.myspace.com/> .

is:pandora
      rdf:type is:InfoService ;
      rdfs:isDefinedBy "http://purl.org/ontology/infoservice/"^^xsd:string ;
      dc:description "An automated music recommendation service."^^xsd:string ;
      dc:title "Pandora"^^xsd:string ;
      foaf:homepage <http://www.pandora.com/> .

is:recommender_service
      rdf:type is:InfoServiceType ;
      rdfs:isDefinedBy "http://purl.org/ontology/infoservice/"^^xsd:string ;
      dc:description "A recommender service forms or works from a specific type of information filtering system technique that attempts to recommend information items (films, television, video on demand, music, books, news, images, web pages, etc) that are likely to be of interest to the user."^^xsd:string ;
      dc:title "recommender service"^^xsd:string .

is:social_network_service
      rdf:type is:InfoServiceType ;
      rdfs:isDefinedBy "http://purl.org/ontology/infoservice/"^^xsd:string ;
      dc:description "A social network service focuses on building and reflecting of social networks or social relations among people, e.g., who share interests and/or activities. A social network service essentially consists of a representation of each user (often a profile), his/her social links, and a variety of additional services."^^xsd:string ;
      dc:title "social network service"^^xsd:string .

is:spotify
      rdf:type is:InfoService ;
      rdfs:isDefinedBy "http://purl.org/ontology/infoservice/"^^xsd:string ;
      dc:description "A proprietary peer-to-peer  music streaming service."^^xsd:string ;
      dc:title "Spotify"^^xsd:string ;
      foaf:homepage <http://www.spotify.com/> .

is:useless
      rdf:type is:InfoServiceQuality ;
      rdfs:isDefinedBy "http://purl.org/ontology/infoservice/"^^xsd:string ;
      dc:description "This is currently worst quality level from the info service quality scale."^^xsd:string ;
      dc:title "useless"^^xsd:string .

is:very_bad
      rdf:type is:InfoServiceQuality ;
      rdfs:isDefinedBy "http://purl.org/ontology/infoservice/"^^xsd:string ;
      dc:description "This is currently second worst quality level from the info service quality scale."^^xsd:string ;
      dc:title "very bad"^^xsd:string .

is:very_good
      rdf:type is:InfoServiceQuality ;
      rdfs:isDefinedBy "http://purl.org/ontology/infoservice/"^^xsd:string ;
      dc:description "This is currently the best quality level from the info service quality scale."^^xsd:string ;
      dc:title "very good"^^xsd:string .

is:wikipedia
      rdf:type is:InfoService ;
      rdfs:isDefinedBy "http://purl.org/ontology/infoservice/"^^xsd:string ;
      dc:description "A free, web-based, collaborative, multilingual encyclopedia project."^^xsd:string ;
      dc:title "Wikipedia"^^xsd:string ;
      foaf:homepage <http://www.wikipedia.org/> .
